LeanMove/Typing/TypeSoundness.lean
@@ -56,16 +56,13 @@ theorem type_soundness_dec (f : FunDef) (lenvDec : LabelEnvDec)
     (args : List Value) (heap : Heap)
     (hcheck : check_fun_dec f lenvDec = true)
     (hfunEnv : checkFunEnv funEnv fte = true)
-    (hdec : SoundnessAssumptions.checkDecidable f lenvDec.toLabelEnv heap = true) :
+    (hdec : SoundnessAssumptions.checkDecidable f lenvDec heap = true) :
     ∀ n loc, Semantics.run n (initState f funEnv args heap) ≠ .error (.danglingRef loc) :=
   type_soundness f lenvDec.toLabelEnv funEnv args heap
     (check_fun_dec_sound f lenvDec hcheck)
     (checkFunEnv_sound funEnv fte hfunEnv)
-    (SoundnessAssumptions.of_check f lenvDec.toLabelEnv heap
+    (SoundnessAssumptions.of_check f lenvDec heap
       (check_fun_dec_lenv_wf f lenvDec hcheck)
-      (check_fun_dec_lenv_non_member_from f lenvDec hcheck)
-      (check_fun_dec_lenv_non_member_to f lenvDec hcheck)
-      (check_fun_dec_lenv_self_loop f lenvDec hcheck)
       hdec)
 
 end LeanMove.Typing.TypeSoundness
